\documentclass{article}
\usepackage[utf8]{inputenc}

\title{RBE 502 HW 1 - Problem 2}
\author{Keith Chester}
\date{August 2021}

\begin{document}

\maketitle

In this problem we look at a system of a 1 dimensional minecart on a frictionless path. Here, the equation for the system is represented as

\[m\dot v = u +\phi(t)\]

where \(u\) is our control system, set to:

\[u=k_p(s-v)+k_d(0-\dot v)=k_ps-k_pv-k_d\dot v\]

which plugged into our systems equation:

\[(m+k_d)\dot v + k_p v = k_p s + \phi(t)\]

We will attempt to find the upperbound for \(\mid v \mid\) as \(t \to \infty\) . To do this, first we shall rewrite our equation in a form of \(\frac{dy}{dt}+ay=g(t)\).

\[\dot v + \frac{k_p v}{m+k_d}= \frac{k_p s + \phi(t)}{m+k_d}\]

...so our resulting function is

\[v = e^{-\frac{k_p}{m+kd}t} \int {e^{\frac{k_p}{m+k_d}t}(\frac{k_p s + \phi(t)}{m + k_d})} \,dt + c_1 e^{-\frac{k_p}{m+kd}t} \]

...and if we expand our integral into two separate integrals: 

\[v = e^{-\frac{k_p}{m+kd}t} \int \frac{e^{\frac{k_p}{m+k_d}t} s k_p}{m+k_d} dt + e^{-\frac{k_p}{m+kd}t} \int \frac{e^{\frac{k_p}{m+k_d}t} \phi(t)}{m + k_d} \,dt + c_1 e^{-\frac{k_p}{m+kd}t}\]

...where we can easily take care of one of the integrals:

\[v = e^{-\frac{k_p}{m+kd}t} e^{\frac{k_p}{m+k_d} t } s + e^{-\frac{k_p}{m+kd}t} \int \frac{e^{\frac{k_p}{m+k_d}t} \phi(t)}{m + k_d} \,dt + c_1 e^{-\frac{k_p}{m+kd}t}\]

...which simplifies down to:

\[v = s + e^{-\frac{k_p}{m+kd}t} \int \frac{e^{\frac{k_p}{m+k_d}t} \phi(t)}{m + k_d} \,dt + c_1 e^{-\frac{k_p}{m+kd}t}\]

From here, we can utilize integration by parts for our remaining integral. For our purposes:

\[\int u v \,dt = u \int v \,dt - \int (\dot u \int v \,dt)\,dt\]

...where \(u = \frac{\phi(t)}{m+k_d}\), \(\dot u = \frac{\dot \phi(t)}{m+k_d}, v = e^{\frac{k_p}{m+k_d}t}\), and \(\int v = \frac{e^{\frac{k_p}{m+k_d}t}(m+k_d)}{k_p}\), thus making our second integral:

\[\frac{\phi(t)}{m+k_d} \frac{e^{\frac{k_p}{m+k_d}t}(m+k_d)}{k_p} - \int { \frac{\dot \phi(t)}{m+k_d} \frac{e^{\frac{k_p}{m+k_d}t}(m+k_d)}{k_p}}\]

which simplifies to

\[ \frac{\phi(t) e^{\frac{k_p}{m+k_d}t}}{kp} - \int \frac{\dot \phi(t) e^{\frac{k_p}{m+k_d}t}}{k_p} \]

When we plug this back into our prior equation:

\[v = s + e^{-\frac{k_p}{m+kd}t} (\frac{\phi(t) e^{\frac{k_p}{m+k_d}t}}{kp} - \int \frac{\dot \phi(t) e^{\frac{k_p}{m+k_d}t}}{k_p}) + c_1 e^{-\frac{k_p}{m+kd}t}\]

which simplifies further to:

\[v = s + \frac{\phi(t)}{kp} - e^{-\frac{k_p}{m+kd}t} \int \frac{\dot \phi(t) e^{\frac{k_p}{m+k_d}t}}{k_p} + c_1 e^{-\frac{k_p}{m+kd}t}\]


We take the limit of our resulting system equation as \(t \to \infty\):

\[\lim_{t \to \infty} v(t) = s + \frac{\phi(t)}{k_p} - e^{-\infty} \int \frac{e^{\infty} \dot \phi(t)}{m+k_d} \,dt + c_1 e^{-\infty}\]

...and since \(e^{-\infty} = 0\):

\[\lim_{t \to \infty} v(t) = s + \frac{\phi(t)}{k_p}\]

Since \(\phi(t) < a\) as per our description, we can thus say that the upperbound velocity of the given problem is defined by

\[v(t) < s + \frac{a}{k_p}\]

\end{document}